- transitivity is done for the new restrcition

proof/uni/def_ott.v
@@ -160,6 +160,13 @@ with open_conts_wrt_exp_rec (k:nat) (e5:exp) (cs5:conts) {struct cs5}: conts :=
   | (conts_sub A) => conts_sub A
 end.
 
+Definition open_dbind_wrt_typ_rec (k:nat) (A5:typ) (db5:dbind) : dbind :=
+  match db5 with
+  | dbind_tvar_empty => dbind_tvar_empty 
+  | dbind_stvar_empty => dbind_stvar_empty 
+  | (dbind_typ A) => dbind_typ (open_typ_wrt_typ_rec k A5 A)
+end.
+
 Definition open_work_wrt_typ_rec (k:nat) (A_5:typ) (w5:work) : work :=
   match w5 with
   | (work_infer e cs) => work_infer (open_exp_wrt_typ_rec k A_5 e) (open_conts_wrt_typ_rec k A_5 cs)
@@ -174,14 +181,6 @@ Definition open_work_wrt_typ_rec (k:nat) (A_5:typ) (w5:work) : work :=
   | (work_unioninfabs A1 B1 A2 B2 cd) => work_unioninfabs (open_typ_wrt_typ_rec k A_5 A1) (open_typ_wrt_typ_rec k A_5 B1) (open_typ_wrt_typ_rec k A_5 A2) (open_typ_wrt_typ_rec k A_5 B2) (open_contd_wrt_typ_rec k A_5 cd)
   | (work_applys cs A) => work_applys (open_conts_wrt_typ_rec k A_5 cs) (open_typ_wrt_typ_rec k A_5 A)
   | (work_applyd cd A B) => work_applyd (open_contd_wrt_typ_rec k A_5 cd) (open_typ_wrt_typ_rec k A_5 A) (open_typ_wrt_typ_rec k A_5 B)
-end.
-
-Definition open_abind_wrt_typ_rec (k:nat) (A5:typ) (ab5:abind) : abind :=
-  match ab5 with
-  | abind_tvar_empty => abind_tvar_empty 
-  | abind_stvar_empty => abind_stvar_empty 
-  | abind_etvar_empty => abind_etvar_empty 
-  | (abind_var_typ A) => abind_var_typ (open_typ_wrt_typ_rec k A5 A)
 end.
 
 Definition open_work_wrt_exp_rec (k:nat) (e5:exp) (w5:work) : work :=
@@ -200,25 +199,12 @@ Definition open_work_wrt_exp_rec (k:nat) (e5:exp) (w5:work) : work :=
   | (work_applyd cd A B) => work_applyd (open_contd_wrt_exp_rec k e5 cd) A B
 end.
 
-Definition open_dbind_wrt_typ_rec (k:nat) (A5:typ) (db5:dbind) : dbind :=
-  match db5 with
-  | dbind_tvar_empty => dbind_tvar_empty 
-  | dbind_stvar_empty => dbind_stvar_empty 
-  | (dbind_typ A) => dbind_typ (open_typ_wrt_typ_rec k A5 A)
-end.
-
-Fixpoint open_aworklist_wrt_typ_rec (k:nat) (A5:typ) (Γ_5:aworklist) {struct Γ_5}: aworklist :=
-  match Γ_5 with
-  | aworklist_empty => aworklist_empty 
-  | (aworklist_cons_var Γ X ab) => aworklist_cons_var (open_aworklist_wrt_typ_rec k A5 Γ) X (open_abind_wrt_typ_rec k A5 ab)
-  | (aworklist_cons_work Γ w) => aworklist_cons_work (open_aworklist_wrt_typ_rec k A5 Γ) (open_work_wrt_typ_rec k A5 w)
-end.
-
-Fixpoint open_aworklist_wrt_exp_rec (k:nat) (e5:exp) (Γ_5:aworklist) {struct Γ_5}: aworklist :=
-  match Γ_5 with
-  | aworklist_empty => aworklist_empty 
-  | (aworklist_cons_var Γ X ab) => aworklist_cons_var (open_aworklist_wrt_exp_rec k e5 Γ) X ab
-  | (aworklist_cons_work Γ w) => aworklist_cons_work (open_aworklist_wrt_exp_rec k e5 Γ) (open_work_wrt_exp_rec k e5 w)
+Definition open_abind_wrt_typ_rec (k:nat) (A5:typ) (ab5:abind) : abind :=
+  match ab5 with
+  | abind_tvar_empty => abind_tvar_empty 
+  | abind_stvar_empty => abind_stvar_empty 
+  | abind_etvar_empty => abind_etvar_empty 
+  | (abind_var_typ A) => abind_var_typ (open_typ_wrt_typ_rec k A5 A)
 end.
 
 Fixpoint open_dworklist_wrt_typ_rec (k:nat) (A5:typ) (Ω5:dworklist) {struct Ω5}: dworklist :=
@@ -235,19 +221,19 @@ Fixpoint open_dworklist_wrt_exp_rec (k:nat) (e5:exp) (Ω5:dworklist) {struct Ω5
   | (dworklist_cons_work Ω w) => dworklist_cons_work (open_dworklist_wrt_exp_rec k e5 Ω) (open_work_wrt_exp_rec k e5 w)
 end.
 
-Definition open_typ_wrt_typ A_5 A__6 := open_typ_wrt_typ_rec 0 A__6 A_5.
+Fixpoint open_aworklist_wrt_typ_rec (k:nat) (A5:typ) (Γ_5:aworklist) {struct Γ_5}: aworklist :=
+  match Γ_5 with
+  | aworklist_empty => aworklist_empty 
+  | (aworklist_cons_var Γ X ab) => aworklist_cons_var (open_aworklist_wrt_typ_rec k A5 Γ) X (open_abind_wrt_typ_rec k A5 ab)
+  | (aworklist_cons_work Γ w) => aworklist_cons_work (open_aworklist_wrt_typ_rec k A5 Γ) (open_work_wrt_typ_rec k A5 w)
+end.
 
-Definition open_contd_wrt_exp e5 cd5 := open_contd_wrt_exp_rec 0 cd5 e5.
-
-Definition open_contd_wrt_typ A5 cd5 := open_contd_wrt_typ_rec 0 cd5 A5.
-
-Definition open_aworklist_wrt_typ A5 Γ_5 := open_aworklist_wrt_typ_rec 0 Γ_5 A5.
-
-Definition open_dbind_wrt_typ A5 db5 := open_dbind_wrt_typ_rec 0 db5 A5.
-
-Definition open_exp_wrt_exp e_5 e__6 := open_exp_wrt_exp_rec 0 e__6 e_5.
-
-Definition open_aworklist_wrt_exp e5 Γ_5 := open_aworklist_wrt_exp_rec 0 Γ_5 e5.
+Fixpoint open_aworklist_wrt_exp_rec (k:nat) (e5:exp) (Γ_5:aworklist) {struct Γ_5}: aworklist :=
+  match Γ_5 with
+  | aworklist_empty => aworklist_empty 
+  | (aworklist_cons_var Γ X ab) => aworklist_cons_var (open_aworklist_wrt_exp_rec k e5 Γ) X ab
+  | (aworklist_cons_work Γ w) => aworklist_cons_work (open_aworklist_wrt_exp_rec k e5 Γ) (open_work_wrt_exp_rec k e5 w)
+end.
 
 Definition open_work_wrt_typ A_5 w5 := open_work_wrt_typ_rec 0 w5 A_5.
 
@@ -264,6 +250,20 @@ Definition open_dworklist_wrt_typ A5 Ω5 := open_dworklist_wrt_typ_rec 0 Ω5 A5.
 Definition open_exp_wrt_typ A_5 e_5 := open_exp_wrt_typ_rec 0 e_5 A_5.
 
 Definition open_dworklist_wrt_exp e5 Ω5 := open_dworklist_wrt_exp_rec 0 Ω5 e5.
+
+Definition open_typ_wrt_typ A_5 A__6 := open_typ_wrt_typ_rec 0 A__6 A_5.
+
+Definition open_contd_wrt_exp e5 cd5 := open_contd_wrt_exp_rec 0 cd5 e5.
+
+Definition open_contd_wrt_typ A5 cd5 := open_contd_wrt_typ_rec 0 cd5 A5.
+
+Definition open_aworklist_wrt_typ A5 Γ_5 := open_aworklist_wrt_typ_rec 0 Γ_5 A5.
+
+Definition open_dbind_wrt_typ A5 db5 := open_dbind_wrt_typ_rec 0 db5 A5.
+
+Definition open_exp_wrt_exp e_5 e__6 := open_exp_wrt_exp_rec 0 e__6 e_5.
+
+Definition open_aworklist_wrt_exp e5 Γ_5 := open_aworklist_wrt_exp_rec 0 Γ_5 e5.
 
 (** closing up abstractions *)
 Fixpoint close_typ_wrt_typ_rec (k:nat) (A_5:var) (A__6:typ) {struct A__6}: typ :=
@@ -773,18 +773,18 @@ Fixpoint fvar_in_dworklist (Ω5:dworklist) : vars :=
   | (dworklist_cons_work Ω w) => (fvar_in_dworklist Ω) \u (fvar_in_work w)
 end.
 
-Fixpoint ftvar_in_aworklist (Γ_5:aworklist) : vars :=
-  match Γ_5 with
-  | aworklist_empty => {}
-  | (aworklist_cons_var Γ X ab) => (ftvar_in_aworklist Γ) \u (ftvar_in_abind ab)
-  | (aworklist_cons_work Γ w) => (ftvar_in_aworklist Γ) \u (ftvar_in_work w)
-end.
-
 Fixpoint fvar_in_aworklist (Γ_5:aworklist) : vars :=
   match Γ_5 with
   | aworklist_empty => {}
   | (aworklist_cons_var Γ X ab) => (fvar_in_aworklist Γ)
   | (aworklist_cons_work Γ w) => (fvar_in_aworklist Γ) \u (fvar_in_work w)
+end.
+
+Fixpoint ftvar_in_aworklist (Γ_5:aworklist) : vars :=
+  match Γ_5 with
+  | aworklist_empty => {}
+  | (aworklist_cons_var Γ X ab) => (ftvar_in_aworklist Γ) \u (ftvar_in_abind ab)
+  | (aworklist_cons_work Γ w) => (ftvar_in_aworklist Γ) \u (ftvar_in_work w)
 end.
 
 (** substitutions *)
@@ -1020,53 +1020,31 @@ Inductive neq_all : typ -> Prop :=    (* defn neq_all *)
      lc_typ A2 ->
      neq_all (typ_intersection A1 A2).
 
-(* defns J_sneq_all *)
-Inductive sneq_all : typ -> Prop :=    (* defn sneq_all *)
- | sneq_all__unit : 
-     sneq_all typ_unit
- | sneq_all__top : 
-     sneq_all typ_top
- | sneq_all__bot : 
-     sneq_all typ_bot
- | sneq_all__var : forall (X:typvar),
-     sneq_all (typ_var_f X)
- | sneq_all__arrow : forall (A1 A2:typ),
+(* defns J_d_wneq_all *)
+Inductive d_wneq_all : denv -> typ -> Prop :=    (* defn d_wneq_all *)
+ | d_wneq_all__unit : forall (Ψ:denv),
+     d_wneq_all Ψ typ_unit
+ | d_wneq_all__top : forall (Ψ:denv),
+     d_wneq_all Ψ typ_top
+ | d_wneq_all__var : forall (Ψ:denv) (X:typvar),
+      binds ( X )  ( dbind_tvar_empty ) ( Ψ )  ->
+     d_wneq_all Ψ (typ_var_f X)
+ | d_wneq_all__arrow : forall (Ψ:denv) (A1 A2:typ),
      lc_typ A1 ->
      lc_typ A2 ->
-     sneq_all (typ_arrow A1 A2)
- | sneq_all__union : forall (A1 A2:typ),
-     sneq_all A1 ->
-     sneq_all A2 ->
-     sneq_all (typ_union A1 A2)
- | sneq_all__intersection : forall (A1 A2:typ),
-     sneq_all A1 ->
-     sneq_all A2 ->
-     sneq_all (typ_intersection A1 A2).
-
-(* defns J_wneq_all *)
-Inductive wneq_all : typ -> Prop :=    (* defn wneq_all *)
- | wneq_all__unit : 
-     wneq_all typ_unit
- | wneq_all__top : 
-     wneq_all typ_top
- | wneq_all__var : forall (X:typvar),
-     wneq_all (typ_var_f X)
- | wneq_all__arrow : forall (A1 A2:typ),
-     lc_typ A1 ->
+     d_wneq_all Ψ (typ_arrow A1 A2)
+ | d_wneq_all__union1 : forall (Ψ:denv) (A1 A2:typ),
      lc_typ A2 ->
-     wneq_all (typ_arrow A1 A2)
- | wneq_all__union1 : forall (A1 A2:typ),
-     lc_typ A2 ->
-     wneq_all A1 ->
-     wneq_all (typ_union A1 A2)
- | wneq_all__union2 : forall (A1 A2:typ),
+     d_wneq_all Ψ A1 ->
+     d_wneq_all Ψ (typ_union A1 A2)
+ | d_wneq_all__union2 : forall (Ψ:denv) (A1 A2:typ),
      lc_typ A1 ->
-     wneq_all A2 ->
-     wneq_all (typ_union A1 A2)
- | wneq_all__intersection2 : forall (A1 A2:typ),
-     wneq_all A1 ->
-     wneq_all A2 ->
-     wneq_all (typ_intersection A1 A2).
+     d_wneq_all Ψ A2 ->
+     d_wneq_all Ψ (typ_union A1 A2)
+ | d_wneq_all__intersection2 : forall (Ψ:denv) (A1 A2:typ),
+     d_wneq_all Ψ A1 ->
+     d_wneq_all Ψ A2 ->
+     d_wneq_all Ψ (typ_intersection A1 A2).
 
 (* defns J_neq_intersection *)
 Inductive neq_intersection : typ -> Prop :=    (* defn neq_intersection *)
@@ -1622,6 +1600,6 @@ Inductive a_wf_env : aenv -> Prop :=    (* defn a_wf_env *)
 
 
 (** infrastructure *)
-#[export] Hint Constructors s_in neq_abs neq_all sneq_all wneq_all neq_intersection neq_union neq_bot d_wf_typ d_wf_exp d_wf_tenv d_wf_env d_mono_typ d_wf_conts d_wf_contd d_wf_work d_wf_twl d_wf_wl a_wf_typ a_mono_typ a_wf_exp a_wf_conts a_wf_contd a_wf_work a_wf_wwl a_wf_twl a_wf_wl a_wf_env lc_typ lc_exp lc_contd lc_conts lc_dbind lc_abind lc_work lc_aworklist lc_dworklist : core.
+#[export] Hint Constructors s_in neq_abs neq_all d_wneq_all neq_intersection neq_union neq_bot d_wf_typ d_wf_exp d_wf_tenv d_wf_env d_mono_typ d_wf_conts d_wf_contd d_wf_work d_wf_twl d_wf_wl a_wf_typ a_mono_typ a_wf_exp a_wf_conts a_wf_contd a_wf_work a_wf_wwl a_wf_twl a_wf_wl a_wf_env lc_typ lc_exp lc_contd lc_conts lc_dbind lc_abind lc_work lc_aworklist lc_dworklist : core.
 
 
